some namespacing and better grind annotations for automata equivalences

Cslib/Computability/Automata/Acceptor.lean
@@ -9,9 +9,9 @@ import Cslib.Computability.Languages.Language
 namespace Cslib.Automata
 
 /-- An `Acceptor` is a machine that recognises strings (lists of symbols in an alphabet). -/
-class Acceptor (α : Type _) (Symbol : outParam (Type _)) where
+class Acceptor (A : Type _) (Symbol : outParam (Type _)) where
   /-- Predicate that establishes whether a string `xs` is accepted. -/
-  Accepts (a : α) (xs : List Symbol) : Prop
+  Accepts (a : A) (xs : List Symbol) : Prop
 
 namespace Acceptor
 
@@ -19,12 +19,12 @@ variable {Symbol : Type _}
 
 /-- The language of an `Acceptor` is the set of strings it `Accepts`. -/
 @[scoped grind .]
-def language [Acceptor α Symbol] (a : α) : Language Symbol :=
+def language [Acceptor A Symbol] (a : A) : Language Symbol :=
   { xs | Accepts a xs }
 
 /-- A string is in the language of an acceptor iff the acceptor accepts it. -/
 @[scoped grind =]
-theorem mem_language [Acceptor α Symbol] (a : α) (xs : List Symbol) :
+theorem mem_language [Acceptor A Symbol] (a : A) (xs : List Symbol) :
   xs ∈ language a ↔ Accepts a xs := Iff.rfl
 
 end Acceptor
